a start on gc_move_loop

compiler/backend/proofs/stack_allocProofScript.sml
@@ -380,6 +380,10 @@ val map_bitmap_APPEND_APPEND = prove(
   \\ Cases_on `ws1` \\ full_simp_tac(srw_ss())[LENGTH,map_bitmap_def]
   \\ srw_tac[][] \\ every_case_tac \\ full_simp_tac(srw_ss())[]) |> SIMP_RULE std_ss [];
 
+val word_gc_move_bitmaps_Loc =
+  ``word_gc_move_bitmaps conf (Loc l1 l2,stack,bitmaps,i1,pa1,curr,m,dm)``
+  |> SIMP_CONV std_ss [word_gc_move_bitmaps_def,full_read_bitmap_def];
+
 val word_gc_move_bitmaps_unroll = prove(
   ``LENGTH bitmaps < dimword (:'a) - 1 /\ good_dimindex (:'a) /\
     word_gc_move_bitmaps conf (Word w,stack,bitmaps,i1,pa1,curr,m,dm) = SOME x ==>
@@ -883,11 +887,108 @@ val word_gc_move_list_code_thm = store_thm("word_gc_move_code_thm",
   \\ once_rewrite_tac [split_num_forall_to_10]
   \\ full_simp_tac(srw_ss())[nine_less])
 
+val word_gc_move_loop_code_def = Define `
+  word_gc_move_loop_code conf =
+    While NotEqual 3 (Reg 8)
+     (list_Seq [load_inst 0 8;
+                move 1 0;
+                (* following decodes header h in 1, len in 0 *)
+                right_shift_inst 1 (2 + conf.len_size);
+                right_shift_inst 0 2;
+                clear_top_inst 0 (conf.len_size - 1);
+                If Test 1 (Imm 1w) ARB ARB])`
+
+val (guard_tm,step_tm) = let
+  val tm = word_gc_move_loop_def
+   |> SPEC_ALL |> concl |> rand |> rator |> rator |> rand |> rator
+  in (tm |> rator |> rand, tm |> rand) end
+
+val word_gc_move_loop_OWHILE = prove(
+  ``!x y.
+      OWHILE ^guard_tm ^step_tm x = SOME y ==>
+      !pb1 i1 pa1 old1 m1 dm1 c1 pb2 i2 pa2 old2 m2 dm2 c2 s.
+        (x = (pb1,i1,pa1,old1,m1,dm1,c1)) /\
+        (y = (pb2,i2,pa2,old2,m2,dm2,c2)) /\
+        shift_length conf < dimindex (:'a) /\ word_shift (:'a) < dimindex (:'a) /\
+        2 < dimindex (:'a) /\ conf.len_size <> 0 /\
+        (!w:'a word. w << word_shift (:'a) = w * bytes_in_word) /\
+        FLOOKUP s.store CurrHeap = SOME (Word old1) /\ s.use_store /\
+        s.memory = m1 /\ s.mdomain = dm1 /\
+        0 IN FDOM s.regs /\
+        1 IN FDOM s.regs /\
+        2 IN FDOM s.regs /\
+        get_var 3 s = SOME (Word pa1) /\
+        get_var 4 s = SOME (Word (i1:'a word)) /\
+        5 IN FDOM s.regs ==>
+        6 IN FDOM s.regs ==>
+        7 IN FDOM s.regs ==>
+        get_var 8 s = SOME (Word pb1) /\ c1 /\ c2 ==>
+        ?ck r0 r1 r2 r5 r6 r7.
+          evaluate (word_gc_move_loop_code conf,s with clock := s.clock + ck) =
+            (NONE,s with <| memory := m1;
+                            regs := s.regs |++ [(0,r0);
+                                                (1,r1);
+                                                (2,r2);
+                                                (3,Word pa2);
+                                                (4,Word i2);
+                                                (5,r5);
+                                                (6,r6);
+                                                (7,r7);
+                                                (8,Word pb2)] |>)``,
+  HO_MATCH_MP_TAC whileTheory.OWHILE_IND \\ rpt strip_tac
+  THEN1 (fs [] \\ rpt var_eq_tac
+    \\ fs [word_gc_move_loop_code_def,get_var_def] \\ tac
+    \\ full_simp_tac(srw_ss())[state_component_equality]
+    \\ full_simp_tac(srw_ss())[FUPDATE_LIST,GSYM fmap_EQ,FLOOKUP_DEF,EXTENSION,
+           FUN_EQ_THM,FAPPLY_FUPDATE_THM]
+    \\ once_rewrite_tac [split_num_forall_to_10]
+    \\ full_simp_tac(srw_ss())[nine_less])
+  \\ rpt var_eq_tac \\ fs []
+  \\ cheat);
+
+val OOWHILE_def = Define `
+  OOWHILE g f x =
+    case OWHILE (\x. case x of NONE => F | SOME y => g y)
+           (\x. case x of NONE => NONE
+                        | SOME y => f y) (SOME x) of
+    | NONE => NONE
+    | SOME NONE => NONE
+    | SOME (SOME x) => SOME x`
+
+val OOWHILE_THM = prove(
+  ``OOWHILE g f x =
+      if g x then
+        (case f x of
+         | NONE => NONE
+         | SOME y => OOWHILE g f y)
+      else SOME x``,
+  simp [Once OOWHILE_def]
+  \\ once_rewrite_tac [whileTheory.OWHILE_THM]
+  \\ rewrite_tac [OOWHILE_def]
+  \\ fs [] \\ rw []
+  \\ Cases_on `f x` \\ fs []
+  \\ once_rewrite_tac [whileTheory.OWHILE_THM]
+  \\ fs []);
+
+val OOWHILE_IND = prove(
+  ``∀P G f.
+     (∀s. ¬G s ⇒ P s s) ∧
+     (∀s1 si s2. G s1 /\ f s1 = SOME si ∧ P si s2 ⇒ P s1 s2) ⇒
+     ∀s1 s2. OOWHILE G f s1 = SOME s2 ⇒ P s1 s2``,
+  cheat);
+
+
+
+
+
+
 (*
 
 word_gc_move_loop_eq
 word_gc_move_bitmap_unroll
 word_gc_move_bitmaps_unroll
+word_gc_move_roots_bitmaps
+gc_thm
 
 *)
 
